Checkpoint

src/tls/Cert.fst
@@ -47,13 +47,34 @@ let verify_signature c pv nonces_or_log csa sigalgs tbs sigv =
         let algs : list sigHashAlg =
           match sigalgs with
           | Some l -> l
+          // This is the RFC default, but I'm tempted to go non-standard here and add SHA256 anyway
           | None -> [(sa, Hash CoreCrypto.SHA1)] in
         if List.Tot.existsb (fun (xs,xh)->(xs=sa && xh=Hash h)) algs then
           CoreCrypto.cert_verify_sig (List.Tot.hd c) sa h tbs sigv
         else false
      | _ -> false)
     else false
-  | _ -> false // TODO!!
+  | _ -> false // TODO! New signature format in 4.8.1
+
+val lookup_server_chain: config -> protocolVersion -> option sigAlg -> negotiatedExtensions -> Tot (result (chain * Sig.skey * list sigHashAlg))
+let lookup_server_chain cfg pv sa ne =
+  let sal = if is_None sa then None else
+    Some (match ne.ne_signature_algorithms with
+    | None ->
+       let sa = Some.v sa in
+       (match pv with
+       | TLS_1p3 -> Error(AD_missing_extension, perror __SOURCE_FILE__ __LINE__ "missing supported signature algorithm extension in a 1.3 signature-based ciphersuite") // 6.3.2.1 of TLS 1.3 requires sending the "missing extension" alert 
+       | _ -> [sa, Hash CoreCrypto.SHA1])
+               // This doesn't comply with 7.4.1.4.1. of RFC5246
+               // which requires selecting RSASIG regardless of the CS's sigAlg
+               // (thus enabling the use of ECDHE_ECDSA with RSA cert if extension is omitted)
+    | Some al -> List.Tot.filter (fun (s,_)->s=sa) al) in
+  match CoreCrypto.cert_load_chain cfg.cert_chain_file cfg.private_key_file with
+  | Some (chain, sk) ->
+    let sk = match sk with 
+  | None -> Eror(AD_no_certificate, perror __SOURCE_FILE__ __LINE__ "cannot find suitable server certificate")
+
+//let certificate_sign: chain -> 
 
 (*
 type sign_cert = option (chain * Sig.alg * Sig.skey)
